src/matroid/scratch.lean
@@ -1,0 +1,17 @@
+
+import tactic
+
+def divides (a b : ℕ) : Prop :=  ∃ d, a*d = b 
+
+def prime (p : ℕ) : Prop := (1 < p) ∧ (∀ x, divides x p → x = 1 ∨ x = p)
+
+lemma even_not_prime (x : ℕ) (h : 1 < x) : ¬ prime (2*x) := 
+λ h', (h'.2 2 ⟨_,rfl⟩).elim (λ _, by linarith) (λ _, h.ne (by linarith))
+
+
+lemma foo (α : Type) (s t : set α) (h_squirrel : s.finite) (ht : t.finite) : 
+  (s ∪ t).finite := 
+ h_squirrel.union ht
+-- begin
+--   exact set.finite.union hs ht, 
+-- end 
